src/generatedproof/kubernetes_model/apimodel.v
@@ -26,6 +26,8 @@ Require Export New.generatedproof.k8s_io.kubernetes.pkg.apis.core.
 Require Export New.generatedproof.k8s_io.kubernetes.pkg.apis.core.v1.
 Require Export New.generatedproof.k8s_io.kubernetes.pkg.controller.
 Require Export New.generatedproof.k8s_io.kubernetes.pkg.registry.apps.replicaset.
+Require Export New.generatedproof.k8s_io.kubernetes.pkg.registry.apps.statefulset.
+Require Export New.generatedproof.k8s_io.kubernetes.pkg.registry.core.persistentvolumeclaim.
 Require Export New.generatedproof.k8s_io.kubernetes.pkg.registry.core.pod.
 Require Export New.generatedproof.math.rand.
 Require Export New.generatedproof.reflect.
