src/proof/kubernetes_model/get.v
@@ -247,8 +247,7 @@ Proof.
     with "[$Hinit $Hisk $Hown_meta_frag $Hown_spec_frag $Hown_status_frag]").
   iIntros (i kobj) "Hpost". iNamed "Hpost".
   iDestruct "Hpost" as "((Hown_spec_frag & %Hspec_eq) & Hown_status_frag & %Hstatus_eq)".
-  destruct kobj as [pod|rs].
-  2: { simpl in Hspec_eq. done. }
+  destruct kobj as [pod|rs|pvc|sts]; try solve [simpl in Hspec_eq; done].
   simpl in Hvalid', Hkey_eq, Hmeta_eq, Hspec_eq, Hstatus_eq.
   assert (Hspec_eq' : kspec = pod.(PodV.Spec')) by congruence.
   assert (Hstatus_eq' : kstatus = pod.(PodV.Status')) by congruence.
@@ -334,8 +333,7 @@ Proof.
     with "[$Hinit $Hisk $Hown_meta_frag $Hown_spec_frag]").
   iIntros (i kobj) "Hpost". iNamed "Hpost".
   iDestruct "Hpost" as "((Hown_spec_frag & %Hspec_eq) & _)".
-  destruct kobj as [pod|rs].
-  { simpl in Hspec_eq. done. }
+  destruct kobj as [pod|rs|pvc|sts]; try solve [simpl in Hspec_eq; done].
   simpl in Hvalid', Hkey_eq, Hmeta_eq, Hspec_eq.
   assert (Hspec_eq' : kspec = rs.(ReplicaSetV.Spec')) by congruence.
   clear Hspec_eq.
